Fix lemmas for basic pattern "dual_since", add requirements for example "Smart lighting", add program for example "Barrier"

examples/SmartLighting/CommonExtraInv.thy
@@ -8,9 +8,9 @@ definition commonExtraInv where "commonExtraInv s== toEnvP s \<and>
 (getPstate s p_Motion' = STOP \<longrightarrow> getVarBool s v_turnedOn' = False) \<and>
 (getPstate s p_Motion' = p_Motion's_movement' \<longrightarrow> ltime s p_Motion' \<le> v_LIGHTING_TIME'TIMEOUT) \<and>
 getPstate s p_Motion' \<in> {p_Motion's_noMovement', p_Motion's_movement', STOP} \<and>
-(getPstate s p_Lighting' = p_Lighting's_night' \<longrightarrow> getVarBool s v_dayLight' = False \<and> getVarBool s v_dimLight' = False \<and>
+(getPstate s p_Lighting' \<in>{ p_Lighting's_night', STOP} \<longrightarrow> getVarBool s v_dayLight' = False \<and> getVarBool s v_dimLight' = False \<and>
    getVarInt s v_timeOfDay' = v_NIGHT') \<and>
-(getPstate s p_Lighting' = p_Lighting's_night' \<longrightarrow> getPstate s p_Motion' = STOP) \<and>
+(getPstate s p_Lighting'  \<in>{ p_Lighting's_night', STOP} \<longrightarrow> getPstate s p_Motion' = STOP) \<and>
 (getPstate s p_Lighting' \<notin> {p_Lighting's_night', STOP} \<longrightarrow> getPstate s p_Motion' \<noteq> STOP) \<and>
 (getPstate s p_Lighting' = p_Lighting's_earlyMorning' \<longrightarrow> getVarBool s v_dayLight' = False \<and> getVarInt s v_timeOfDay' = v_EARLY_MORNING') \<and>
 (getPstate s p_Lighting' = p_Lighting's_morningLighting' \<longrightarrow> getVarBool s v_dimLight' = True \<and> getVarBool s v_dayLight' = False \<and>
