examples/Barrier/Barrier.thy
@@ -1,0 +1,27 @@
+theory Barrier imports VCProving.VCTheory
+begin
+
+abbreviation v_carInFront' :: variable where "v_carInFront' \<equiv> (Suc 0)"
+abbreviation v_peCarUnder' :: variable where "v_peCarUnder' \<equiv> (Suc (Suc 0))"
+abbreviation v_opened' :: variable where "v_opened' \<equiv> (Suc (Suc (Suc 0)))"
+abbreviation v_closed' :: variable where "v_closed' \<equiv> (Suc (Suc (Suc (Suc 0))))"
+abbreviation v_up' :: variable where "v_up' \<equiv> (Suc (Suc (Suc (Suc (Suc 0)))))"
+abbreviation v_down' :: variable where "v_down' \<equiv> (Suc (Suc (Suc (Suc (Suc (Suc 0))))))"
+abbreviation v_green' :: variable where "v_green' \<equiv> (Suc (Suc (Suc (Suc (Suc (Suc (Suc 0)))))))"
+abbreviation v_red' :: variable where "v_red' \<equiv> (Suc (Suc (Suc (Suc (Suc (Suc (Suc (Suc 0))))))))"
+
+abbreviation p_CarController' :: process where "p_CarController' \<equiv> (Suc 0)"
+abbreviation p_Opening' :: process where "p_Opening' \<equiv> (Suc (Suc 0))"
+
+abbreviation p_CarController's_waitingForCarPassing' :: pstate where "p_CarController's_waitingForCarPassing' \<equiv> (Suc (Suc (Suc 0)))"
+abbreviation p_CarController's_waitingForCar' :: pstate where "p_CarController's_waitingForCar' \<equiv> (Suc (Suc 0))"
+abbreviation p_Opening's_closing' :: pstate where "p_Opening's_closing' \<equiv> (Suc (Suc (Suc (Suc (Suc (Suc 0))))))"
+abbreviation p_Opening's_opening' :: pstate where "p_Opening's_opening' \<equiv> (Suc (Suc (Suc (Suc 0))))"
+abbreviation p_Opening's_open' :: pstate where "p_Opening's_open' \<equiv> (Suc (Suc (Suc (Suc (Suc 0)))))"
+
+abbreviation v_OPEN_TIME' :: nat where "v_OPEN_TIME' \<equiv> 600000"
+
+abbreviation v_OPEN_TIME'TIMEOUT :: nat where "v_OPEN_TIME'TIMEOUT \<equiv> 6000"
+
+end
+
