examples/Barrier/ExtraInv_R4.thy
@@ -1,0 +1,438 @@
+theory ExtraInv_R4
+  imports CommonExtraInv Requirements
+begin
+
+definition R4Pattern_inv where "R4Pattern_inv s t t1 b1 b2 A1 A2 A3 A4 A5 A6 A7 \<equiv> 
+P1'inv s t t1 A1 (\<lambda> s2. (previous_all s2 A2 \<or> A3 s2) \<and> A4 s2) (\<lambda> s3. (previous_ex s3 A5 \<and> A6 s3) \<or> A7 s3) \<and>
+(b1 \<longrightarrow> A2 s) \<and> (b2 \<longrightarrow> A5 s)"
+
+lemma R4Pattern_rule: "
+ R4Pattern_inv s0 t t1 b1 b2 A1 A2 A3 A4 A5 A6 A7 \<Longrightarrow>
+((\<not> A1 s \<or> (b2 \<and> A6 s \<or> A7 s) \<or> ((b1 \<or> A3 s) \<and> A4 s) \<and> t2 > 0)  \<and>
+(t1 = 0 \<or> (b2 \<and> A6 s \<or> A7 s) \<and> t1 \<le> t \<or> ((b1 \<or> A3 s) \<and> A4 s)  \<and> t1 < t2)) \<and>
+(b1' \<longrightarrow> A2 s)\<and> (b2' \<longrightarrow> A5 s) \<Longrightarrow>
+consecutive s0 s \<Longrightarrow>
+ R4Pattern_inv s t t2 b1' b2' A1 A2 A3 A4 A5 A6 A7"
+apply( unfold R4Pattern_inv_def)
+ (* using P1'inv_rule1 previous_ex_one_point previous_all_one_point
+  by (smt (z3))
+*)
+  apply(erule conjE)
+  apply(erule conjE)
+  subgoal premises prems1
+    apply(rule conjI)
+     apply(insert prems1(1,2,4))[1]
+     apply(erule P1'inv_rule_gen)
+      apply simp
+     apply(erule conjE)
+    subgoal premises prems2
+      apply(rule conjI)
+       apply(insert prems2(1,2))[1]
+       apply(erule disjE)
+        apply(rule disjI1)
+        apply simp
+       apply(rule disjI2)
+       apply(erule disjE)
+        apply(rule disjI1)
+        apply(erule disjE)
+         apply(rule disjI1)
+         apply(erule conjE)
+      subgoal premises prems3
+        apply(rule conjI)
+         apply(insert prems3(1,2))[1]
+         apply(rule previous_ex_one_point[of s0])
+          apply simp
+         apply (simp add: prems1(3))
+        apply(insert prems3(1,3))
+        apply simp
+        done
+        apply(rule disjI2)
+        apply simp
+       apply(rule disjI2)
+       apply(erule conjE)
+      subgoal premises prems3
+        apply(rule conjI)
+         apply(insert prems3(1,2))[1]
+         apply(erule conjE)
+        subgoal premises prems4
+          apply(rule conjI)
+           apply(insert prems4(1,2))[1]
+           apply(erule disjE)
+            apply(rule disjI1)
+            apply(rule previous_all_one_point[of s0])
+             apply simp
+            apply (simp add: prems1(3))
+           apply(rule disjI2)
+           apply simp
+          apply(insert prems4(1,3))
+          apply simp
+          done
+        apply(insert prems3(1,3))
+        apply simp
+        done
+      apply(insert prems2(1,3))
+      apply(rule conjI)
+       apply simp
+      apply(rule conjI)
+       apply simp
+      apply(erule disjE)
+       apply(rule disjI1)
+       apply simp
+      apply(rule disjI2)
+      apply(erule disjE)
+       apply(rule disjI1)
+       apply(erule conjE)
+      subgoal premises prems3
+        apply(rule conjI)
+         apply(insert prems3(1,2))[1]
+         apply(erule disjE)
+          apply(rule disjI1)
+          apply(erule conjE)
+        subgoal premises prems4
+          apply(rule conjI)
+           apply(insert prems4(1,2))[1]
+           apply(rule previous_ex_one_point[of s0])
+            apply simp
+           apply (simp add: prems1(3))
+          apply(insert prems4(1,3))
+          apply simp
+          done
+         apply(rule disjI2)
+         apply simp
+        apply(insert prems3(1,3))
+        apply simp
+        done
+      apply(rule disjI2)
+      apply(erule conjE)
+      subgoal premises prems3
+        apply(rule conjI)
+         apply(insert prems3(1,2))[1]
+         apply(erule conjE)
+        subgoal premises prems4
+          apply(rule conjI)
+           apply(insert prems4(1,2))[1]
+           apply(erule disjE)
+            apply(rule disjI1)
+            apply(rule previous_all_one_point[of s0])
+             apply simp
+            apply (simp add: prems1(3))
+           apply(rule disjI2)
+           apply simp
+          apply(insert prems4(1,3))
+          apply simp
+          done
+        apply(insert prems3(1,3))
+        apply simp
+        done
+      done
+    apply(insert prems1(1,3,5))
+    apply simp
+    done
+  done
+
+lemma R4Pattern_einv2req: "R4Pattern_inv s t t1 b1 b2 A1 A2 A3 A4 A5 A6 A7 \<Longrightarrow> t1 \<le> t \<Longrightarrow> R4Pattern s t A1 A2 A3 A4 A5 A6 A7"
+  apply(unfold R4Pattern_def R4Pattern_inv_def)
+  using P1'einv2req_gen
+  by force
+
+definition extraInv where "extraInv s \<equiv> commonExtraInv s \<and>
+R4Pattern_inv s (OPEN_TIME'TIMEOUT) (if getPstate s Opening' = Opening'open' then ltime s Opening' else 0)
+ (getPstate s CarController' = CarController'waitingForCarPassing') (getPstate s CarController' = CarController'waitingForCar')
+ (\<lambda> s1. getVarBool s1 green' = True) (\<lambda> s2. getVarBool s2 carInFront' = True) (\<lambda> s3. getVarBool s3 carInFront' = False)
+(\<lambda> s4. getVarBool s4 down' = False \<and> getVarBool s4 opened' = True \<and> getVarBool s4 peCarUnder' = False) 
+(\<lambda> s2. getVarBool s2 carInFront' = False) (\<lambda> s3. getVarBool s3 carInFront' = True)
+(\<lambda> s4. getVarBool s4 down' = True \<or> getVarBool s4 opened' = False \<or> getVarBool s4 peCarUnder' = True)"
+
+theorem extra1: "VC1 extraInv s0"
+  apply(unfold VC1_def extraInv_def commonExtraInv_def R4Pattern_inv_def P1'inv_def always_def constrained_until_def previous_all_def previous_ex_def)
+  apply auto
+  done
+
+
+theorem extra2: "VC2 extraInv env s0 carInFront'value peCarUnder'value opened'value closed'value"
+apply(unfold VC2_def extraInv_def)
+ apply(rule impI)
+  apply(rule conjI)
+  using cei2 VC2_def apply auto[1]
+  apply(unfold commonExtraInv_def)
+  apply(erule conjE)+
+  apply(erule R4Pattern_rule)
+   apply(auto split: if_splits)
+  done
+
+theorem extra3: "VC3 extraInv env s0 carInFront'value peCarUnder'value opened'value closed'value"
+apply(unfold VC3_def extraInv_def)
+ apply(rule impI)
+  apply(rule conjI)
+  using cei3 VC3_def apply auto[1]
+  apply(unfold commonExtraInv_def)
+  apply(erule conjE)+
+  apply(erule R4Pattern_rule)
+   apply(auto split: if_splits)
+  done
+
+theorem extra4: "VC4 extraInv env s0 carInFront'value peCarUnder'value opened'value closed'value"
+apply(unfold VC4_def extraInv_def)
+ apply(rule impI)
+  apply(rule conjI)
+  using cei4 VC4_def apply auto[1]
+  apply(unfold commonExtraInv_def)
+  apply(erule conjE)+
+  apply(erule R4Pattern_rule)
+   apply(auto split: if_splits)
+  done
+
+theorem extra14: "VC14 extraInv env s0 carInFront'value peCarUnder'value opened'value closed'value"
+apply(unfold VC14_def extraInv_def)
+ apply(rule impI)
+  apply(rule conjI)
+  using cei14 VC14_def apply auto[1]
+  apply(unfold commonExtraInv_def)
+  apply(erule conjE)+
+  apply(erule R4Pattern_rule)
+   apply(auto split: if_splits)
+  done
+
+theorem extra15: "VC15 extraInv env s0 carInFront'value peCarUnder'value opened'value closed'value"
+apply(unfold VC15_def extraInv_def)
+ apply(rule impI)
+  apply(rule conjI)
+  using cei15 VC15_def apply auto[1]
+  apply(unfold commonExtraInv_def)
+  apply(erule conjE)+
+  apply(erule R4Pattern_rule)
+   apply(auto split: if_splits)
+  done
+
+theorem extra16: "VC16 extraInv env s0 carInFront'value peCarUnder'value opened'value closed'value"
+apply(unfold VC16_def extraInv_def)
+ apply(rule impI)
+  apply(rule conjI)
+  using cei16 VC16_def apply auto[1]
+  apply(unfold commonExtraInv_def)
+  apply(erule conjE)+
+  apply(erule R4Pattern_rule)
+   apply(auto split: if_splits)
+  done
+
+theorem extra17: "VC17 extraInv env s0 carInFront'value peCarUnder'value opened'value closed'value"
+apply(unfold VC17_def extraInv_def)
+ apply(rule impI)
+  apply(rule conjI)
+  using cei17 VC17_def apply auto[1]
+  apply(unfold commonExtraInv_def)
+  apply(erule conjE)+
+  apply(erule R4Pattern_rule)
+   apply(auto split: if_splits)
+  done
+
+theorem extra18: "VC18 extraInv env s0 carInFront'value peCarUnder'value opened'value closed'value"
+apply(unfold VC18_def extraInv_def)
+ apply(rule impI)
+  apply(rule conjI)
+  using cei18 VC18_def apply auto[1]
+  apply(unfold commonExtraInv_def)
+  apply(erule conjE)+
+  apply(erule R4Pattern_rule)
+   apply(auto split: if_splits)
+  done
+
+theorem extra19: "VC19 extraInv env s0 carInFront'value peCarUnder'value opened'value closed'value"
+apply(unfold VC19_def extraInv_def)
+ apply(rule impI)
+  apply(rule conjI)
+  using cei19 VC19_def apply auto[1]
+  apply(unfold commonExtraInv_def)
+  apply(erule conjE)+
+  apply(erule R4Pattern_rule)
+   apply(auto split: if_splits)
+  done
+
+theorem extra20: "VC20 extraInv env s0 carInFront'value peCarUnder'value opened'value closed'value"
+apply(unfold VC20_def extraInv_def)
+ apply(rule impI)
+  apply(rule conjI)
+  using cei20 VC20_def apply auto[1]
+  apply(unfold commonExtraInv_def)
+  apply(erule conjE)+
+  apply(erule R4Pattern_rule)
+   apply(auto split: if_splits)
+  done
+
+theorem extra21: "VC21 extraInv env s0 carInFront'value peCarUnder'value opened'value closed'value"
+apply(unfold VC21_def extraInv_def)
+ apply(rule impI)
+  apply(rule conjI)
+  using cei21 VC21_def apply auto[1]
+  apply(unfold commonExtraInv_def)
+  apply(erule conjE)+
+  apply(erule R4Pattern_rule)
+   apply(auto split: if_splits)
+  done
+
+theorem extra22: "VC22 extraInv env s0 carInFront'value peCarUnder'value opened'value closed'value"
+apply(unfold VC22_def extraInv_def)
+ apply(rule impI)
+  apply(rule conjI)
+  using cei22 VC22_def apply auto[1]
+  apply(unfold commonExtraInv_def)
+  apply(erule conjE)+
+  apply(erule R4Pattern_rule)
+   apply(auto split: if_splits)
+  done
+
+theorem extra23: "VC23 extraInv env s0 carInFront'value peCarUnder'value opened'value closed'value"
+apply(unfold VC23_def extraInv_def)
+ apply(rule impI)
+  apply(rule conjI)
+  using cei23 VC23_def apply auto[1]
+  apply(unfold commonExtraInv_def)
+  apply(erule conjE)+
+  apply(erule R4Pattern_rule)
+   apply(auto split: if_splits)
+  done
+
+theorem extra24: "VC24 extraInv env s0 carInFront'value peCarUnder'value opened'value closed'value"
+apply(unfold VC24_def extraInv_def)
+ apply(rule impI)
+  apply(rule conjI)
+  using cei24 VC24_def apply auto[1]
+  apply(unfold commonExtraInv_def)
+  apply(erule conjE)+
+  apply(erule R4Pattern_rule)
+   apply(auto split: if_splits)
+  done
+
+theorem extra25: "VC25 extraInv env s0 carInFront'value peCarUnder'value opened'value closed'value"
+apply(unfold VC25_def extraInv_def)
+ apply(rule impI)
+  apply(rule conjI)
+  using cei25 VC25_def apply auto[1]
+  apply(unfold commonExtraInv_def)
+  apply(erule conjE)+
+  apply(erule R4Pattern_rule)
+   apply(auto split: if_splits)
+  done
+
+theorem extra26: "VC26 extraInv env s0 carInFront'value peCarUnder'value opened'value closed'value"
+apply(unfold VC26_def extraInv_def)
+ apply(rule impI)
+  apply(rule conjI)
+  using cei26 VC26_def apply auto[1]
+  apply(unfold commonExtraInv_def)
+  apply(erule conjE)+
+  apply(erule R4Pattern_rule)
+   apply(auto split: if_splits)
+  done
+
+theorem extra27: "VC27 extraInv env s0 carInFront'value peCarUnder'value opened'value closed'value"
+apply(unfold VC27_def extraInv_def)
+ apply(rule impI)
+  apply(rule conjI)
+  using cei27 VC27_def apply auto[1]
+  apply(unfold commonExtraInv_def)
+  apply(erule conjE)+
+  apply(erule R4Pattern_rule)
+   apply(auto split: if_splits)
+  done
+
+theorem extra28: "VC28 extraInv env s0 carInFront'value peCarUnder'value opened'value closed'value"
+apply(unfold VC28_def extraInv_def)
+ apply(rule impI)
+  apply(rule conjI)
+  using cei28 VC28_def apply auto[1]
+  apply(unfold commonExtraInv_def)
+  apply(erule conjE)+
+  apply(erule R4Pattern_rule)
+   apply(auto split: if_splits)
+  done
+
+theorem extra29: "VC29 extraInv env s0 carInFront'value peCarUnder'value opened'value closed'value"
+apply(unfold VC29_def extraInv_def)
+ apply(rule impI)
+  apply(rule conjI)
+  using cei29 VC29_def apply auto[1]
+  apply(unfold commonExtraInv_def)
+  apply(erule conjE)+
+  apply(erule R4Pattern_rule)
+   apply(auto split: if_splits)
+  done
+
+theorem extra30: "VC30 extraInv env s0 carInFront'value peCarUnder'value opened'value closed'value"
+apply(unfold VC30_def extraInv_def)
+ apply(rule impI)
+  apply(rule conjI)
+  using cei30 VC30_def apply auto[1]
+  apply(unfold commonExtraInv_def)
+  apply(erule conjE)+
+  apply(erule R4Pattern_rule)
+   apply(auto split: if_splits)
+  done
+
+theorem extra31: "VC31 extraInv env s0 carInFront'value peCarUnder'value opened'value closed'value"
+apply(unfold VC31_def extraInv_def)
+ apply(rule impI)
+  apply(rule conjI)
+  using cei31 VC31_def apply auto[1]
+  apply(unfold commonExtraInv_def)
+  apply(erule conjE)+
+  apply(erule R4Pattern_rule)
+   apply(auto split: if_splits)
+  done
+
+theorem extra32: "VC32 extraInv env s0 carInFront'value peCarUnder'value opened'value closed'value"
+apply(unfold VC32_def extraInv_def)
+ apply(rule impI)
+  apply(rule conjI)
+  using cei32 VC32_def apply auto[1]
+  apply(unfold commonExtraInv_def)
+  apply(erule conjE)+
+  apply(erule R4Pattern_rule)
+   apply(auto split: if_splits)
+  done
+
+theorem extra33: "VC33 extraInv env s0 carInFront'value peCarUnder'value opened'value closed'value"
+apply(unfold VC33_def extraInv_def)
+ apply(rule impI)
+  apply(rule conjI)
+  using cei33 VC33_def apply auto[1]
+  apply(unfold commonExtraInv_def)
+  apply(erule conjE)+
+  apply(erule R4Pattern_rule)
+   apply(auto split: if_splits)
+  done
+
+theorem extra34: "VC34 extraInv env s0 carInFront'value peCarUnder'value opened'value closed'value"
+apply(unfold VC34_def extraInv_def)
+ apply(rule impI)
+  apply(rule conjI)
+  using cei34 VC34_def apply auto[1]
+  apply(unfold commonExtraInv_def)
+  apply(erule conjE)+
+  apply(erule R4Pattern_rule)
+   apply(auto split: if_splits)
+  done
+
+theorem extra35: "VC35 extraInv env s0 carInFront'value peCarUnder'value opened'value closed'value"
+apply(unfold VC35_def extraInv_def)
+ apply(rule impI)
+  apply(rule conjI)
+  using cei35 VC35_def apply auto[1]
+  apply(unfold commonExtraInv_def)
+  apply(erule conjE)+
+  apply(erule R4Pattern_rule)
+   apply(auto split: if_splits)
+  done
+
+theorem extra36: "VC36 extraInv env s0 carInFront'value peCarUnder'value opened'value closed'value"
+apply(unfold VC36_def extraInv_def)
+ apply(rule impI)
+  apply(rule conjI)
+  using cei36 VC36_def apply auto[1]
+  apply(unfold commonExtraInv_def)
+  apply(erule conjE)+
+  apply(erule R4Pattern_rule)
+   apply(auto split: if_splits)
+  done
+
+end
