examples/Derived_Patterns.thy
@@ -2283,7 +2283,7 @@ definition P6_1_inv_part where "P6_1_inv_part t b_0 t1_0 b_1 A1 A2 A3 A4 s \<equ
 lemma P6_1_inv_saving_gen: "
 P6_1_inv t b_0 t1_0 b_1 A1 A2 A3 A4_1 s0 \<Longrightarrow>
 consecutive s0 s \<Longrightarrow>
-(((((True \<and> True) \<and> (True \<and> (always_imp s0 (\<lambda> r1 . (A4_1 s0 r1)) (\<lambda> r1 . (A4_1 s r1))))) \<and> (((b_1 s0) \<and> (True \<and> True)) \<or> ((\<not> (A3 s)) \<or> (A4_1 s s)))) \<and> ((b_1 s) --> (((t > 0) \<or> (\<not> (A1 s))) \<and> ((\<not> (A2 s)) \<or> ((b_0 s0) \<and> (True \<and> (True \<and> ((t1_0 s0) < t)))))))) \<and> ((b_0 s) --> ((((t1_0 s) > 0) \<or> (\<not> (A1 s))) \<and> ((\<not> (A2 s)) \<or> ((b_0 s0) \<and> (True \<and> (True \<and> ((t1_0 s0) < (t1_0 s))))))))) \<Longrightarrow>
+(((((True \<and> True) \<and> (True \<and> (always_imp s0 (\<lambda> r1 . (A4_1 s0 r1)) (\<lambda> r1 . (A4_1 s r1))))) \<and> (((b_1 s0) \<and> (True \<and> True)) \<or> ((\<not> (A3 s)) \<or> (A4_1 s s)))) \<and> ((b_1 s) --> (((t > 0) \<or> (\<not> (A1 s))) \<and> ((\<not> (A2 s)) \<or> ((b_0 s0) \<and> (True \<and> (True \<and> ((((t1_0 s0) = 0) \<and> (\<not> (A1 s))) \<or> ((t1_0 s0) < t))))))))) \<and> ((b_0 s) --> ((((t1_0 s) > 0) \<or> (\<not> (A1 s))) \<and> ((\<not> (A2 s)) \<or> ((b_0 s0) \<and> (True \<and> (True \<and> ((((t1_0 s0) = 0) \<and> (\<not> (A1 s))) \<or> ((t1_0 s0) < (t1_0 s)))))))))) \<Longrightarrow>
 P6_1_inv t b_0 t1_0 b_1 A1 A2 A3 A4_1 s"
 
 unfolding P6_1_inv_def
@@ -2404,7 +2404,18 @@ apply(insert prems2(1,3,5))
               apply(insert prems13(1,2))[1]
                 apply(rule always_imp_refl)
               apply(insert prems13(1,3))
-                apply assumption
+                apply(erule disjE)
+                apply(rule disjI1)
+                  apply(erule conjE)
+                  subgoal premises prems14
+                  apply(rule conjI)
+                  apply(insert prems14(1,2))[1]
+                    apply assumption
+                  apply(insert prems14(1,3))
+                    apply assumption
+                  done
+                apply(rule disjI2)
+                  apply assumption
               done
             done
           done
@@ -2417,41 +2428,52 @@ apply(insert prems1(1,3,5))
   apply(rule impI)
   apply(erule impE)
   apply assumption
-  subgoal premises prems14
-  apply(insert prems14(1,3))
+  subgoal premises prems15
+  apply(insert prems15(1,3))
     apply(erule conjE)
-    subgoal premises prems15
+    subgoal premises prems16
     apply(rule conjI)
-    apply(insert prems15(1,2))[1]
+    apply(insert prems16(1,2))[1]
       apply(erule disjE)
       apply(rule disjI1)
         apply assumption
       apply(rule disjI2)
         apply assumption
-    apply(insert prems15(1,3))
+    apply(insert prems16(1,3))
       apply(erule disjE)
       apply(rule disjI1)
         apply assumption
       apply(rule disjI2)
         apply(erule conjE)
-        subgoal premises prems16
+        subgoal premises prems17
         apply(rule conjI)
-        apply(insert prems16(1,2))[1]
+        apply(insert prems17(1,2))[1]
           apply assumption
-        apply(insert prems16(1,3))
+        apply(insert prems17(1,3))
           apply(erule conjE)
-          subgoal premises prems17
+          subgoal premises prems18
           apply(rule conjI)
-          apply(insert prems17(1,2))[1]
+          apply(insert prems18(1,2))[1]
             apply(rule always_imp_refl)
-          apply(insert prems17(1,3))
+          apply(insert prems18(1,3))
             apply(erule conjE)
-            subgoal premises prems18
+            subgoal premises prems19
             apply(rule conjI)
-            apply(insert prems18(1,2))[1]
+            apply(insert prems19(1,2))[1]
               apply(rule always_imp_refl)
-            apply(insert prems18(1,3))
-              apply assumption
+            apply(insert prems19(1,3))
+              apply(erule disjE)
+              apply(rule disjI1)
+                apply(erule conjE)
+                subgoal premises prems20
+                apply(rule conjI)
+                apply(insert prems20(1,2))[1]
+                  apply assumption
+                apply(insert prems20(1,3))
+                  apply assumption
+                done
+              apply(rule disjI2)
+                apply assumption
             done
           done
         done
@@ -2512,7 +2534,7 @@ done
 lemma P6_1_inv_saving: "
 P6_1_inv_part t b_0 t1_0 b_1 A1 A2 A3 A4 s0 \<Longrightarrow>
 consecutive s0 s \<Longrightarrow>
-((((b_1 s0) \<or> ((\<not> (A3 s)) \<or> (A4 s))) \<and> ((b_1 s) --> (((t > 0) \<or> (\<not> (A1 s))) \<and> ((\<not> (A2 s)) \<or> ((b_0 s0) \<and> ((t1_0 s0) < t)))))) \<and> ((b_0 s) --> ((((t1_0 s) > 0) \<or> (\<not> (A1 s))) \<and> ((\<not> (A2 s)) \<or> ((b_0 s0) \<and> ((t1_0 s0) < (t1_0 s))))))) \<Longrightarrow>
+((((b_1 s0) \<or> ((\<not> (A3 s)) \<or> (A4 s))) \<and> ((b_1 s) --> (((t > 0) \<or> (\<not> (A1 s))) \<and> ((\<not> (A2 s)) \<or> ((b_0 s0) \<and> ((((t1_0 s0) = 0) \<and> (\<not> (A1 s))) \<or> ((t1_0 s0) < t))))))) \<and> ((b_0 s) --> ((((t1_0 s) > 0) \<or> (\<not> (A1 s))) \<and> ((\<not> (A2 s)) \<or> ((b_0 s0) \<and> ((((t1_0 s0) = 0) \<and> (\<not> (A1 s))) \<or> ((t1_0 s0) < (t1_0 s)))))))) \<Longrightarrow>
 P6_1_inv_part t b_0 t1_0 b_1 A1 A2 A3 A4 s"
 
 unfolding P6_1_inv_part_def P6_1_part_def
@@ -2550,7 +2572,7 @@ definition P6_2_inv_part where "P6_2_inv_part t b_0 t1_0 b_1 w_0 A1 A2 A3 A4 A5 
 lemma P6_2_inv_saving_gen: "
 P6_2_inv t b_0 t1_0 b_1 w_0 A1 A2 A3 A4_1 A5_1 s0 \<Longrightarrow>
 consecutive s0 s \<Longrightarrow>
-(((((True \<and> True) \<and> (True \<and> ((always_imp s0 (A4_1 s0) (A4_1 s)) \<and> ((always_imp s0 (A5_1 s0) (A5_1 s)) \<and> ((\<not> (w_0 s0)) \<or> ((A5_1 s s) \<or> ((w_0 s) \<and> (A4_1 s s)))))))) \<and> (((b_1 s0) \<and> (True \<and> True)) \<or> ((\<not> (A3 s)) \<or> ((A5_1 s s) \<or> ((w_0 s) \<and> (A4_1 s s)))))) \<and> ((b_1 s) --> (((t > 0) \<or> (\<not> (A1 s))) \<and> ((\<not> (A2 s)) \<or> ((b_0 s0) \<and> (True \<and> (True \<and> ((t1_0 s0) < t)))))))) \<and> ((b_0 s) --> ((((t1_0 s) > 0) \<or> (\<not> (A1 s))) \<and> ((\<not> (A2 s)) \<or> ((b_0 s0) \<and> (True \<and> (True \<and> ((t1_0 s0) < (t1_0 s))))))))) \<Longrightarrow>
+(((((True \<and> True) \<and> (True \<and> ((always_imp s0 (A4_1 s0) (A4_1 s)) \<and> ((always_imp s0 (A5_1 s0) (A5_1 s)) \<and> ((\<not> (w_0 s0)) \<or> ((A5_1 s s) \<or> ((w_0 s) \<and> (A4_1 s s)))))))) \<and> (((b_1 s0) \<and> (True \<and> True)) \<or> ((\<not> (A3 s)) \<or> ((A5_1 s s) \<or> ((w_0 s) \<and> (A4_1 s s)))))) \<and> ((b_1 s) --> (((t > 0) \<or> (\<not> (A1 s))) \<and> ((\<not> (A2 s)) \<or> ((b_0 s0) \<and> (True \<and> (True \<and> ((((t1_0 s0) = 0) \<and> (\<not> (A1 s))) \<or> ((t1_0 s0) < t))))))))) \<and> ((b_0 s) --> ((((t1_0 s) > 0) \<or> (\<not> (A1 s))) \<and> ((\<not> (A2 s)) \<or> ((b_0 s0) \<and> (True \<and> (True \<and> ((((t1_0 s0) = 0) \<and> (\<not> (A1 s))) \<or> ((t1_0 s0) < (t1_0 s)))))))))) \<Longrightarrow>
 P6_2_inv t b_0 t1_0 b_1 w_0 A1 A2 A3 A4_1 A5_1 s"
 
 unfolding P6_2_inv_def
@@ -2715,7 +2737,18 @@ apply(insert prems2(1,3,5))
               apply(insert prems17(1,2))[1]
                 apply(rule always_imp_refl)
               apply(insert prems17(1,3))
-                apply assumption
+                apply(erule disjE)
+                apply(rule disjI1)
+                  apply(erule conjE)
+                  subgoal premises prems18
+                  apply(rule conjI)
+                  apply(insert prems18(1,2))[1]
+                    apply assumption
+                  apply(insert prems18(1,3))
+                    apply assumption
+                  done
+                apply(rule disjI2)
+                  apply assumption
               done
             done
           done
@@ -2728,41 +2761,52 @@ apply(insert prems1(1,3,5))
   apply(rule impI)
   apply(erule impE)
   apply assumption
-  subgoal premises prems18
-  apply(insert prems18(1,3))
+  subgoal premises prems19
+  apply(insert prems19(1,3))
     apply(erule conjE)
-    subgoal premises prems19
+    subgoal premises prems20
     apply(rule conjI)
-    apply(insert prems19(1,2))[1]
+    apply(insert prems20(1,2))[1]
       apply(erule disjE)
       apply(rule disjI1)
         apply assumption
       apply(rule disjI2)
         apply assumption
-    apply(insert prems19(1,3))
+    apply(insert prems20(1,3))
       apply(erule disjE)
       apply(rule disjI1)
         apply assumption
       apply(rule disjI2)
         apply(erule conjE)
-        subgoal premises prems20
+        subgoal premises prems21
         apply(rule conjI)
-        apply(insert prems20(1,2))[1]
+        apply(insert prems21(1,2))[1]
           apply assumption
-        apply(insert prems20(1,3))
+        apply(insert prems21(1,3))
           apply(erule conjE)
-          subgoal premises prems21
+          subgoal premises prems22
           apply(rule conjI)
-          apply(insert prems21(1,2))[1]
+          apply(insert prems22(1,2))[1]
             apply(rule always_imp_refl)
-          apply(insert prems21(1,3))
+          apply(insert prems22(1,3))
             apply(erule conjE)
-            subgoal premises prems22
+            subgoal premises prems23
             apply(rule conjI)
-            apply(insert prems22(1,2))[1]
+            apply(insert prems23(1,2))[1]
               apply(rule always_imp_refl)
-            apply(insert prems22(1,3))
-              apply assumption
+            apply(insert prems23(1,3))
+              apply(erule disjE)
+              apply(rule disjI1)
+                apply(erule conjE)
+                subgoal premises prems24
+                apply(rule conjI)
+                apply(insert prems24(1,2))[1]
+                  apply assumption
+                apply(insert prems24(1,3))
+                  apply assumption
+                done
+              apply(rule disjI2)
+                apply assumption
             done
           done
         done
@@ -2832,7 +2876,7 @@ done
 lemma P6_2_inv_saving: "
 P6_2_inv_part t b_0 t1_0 b_1 w_0 A1 A2 A3 A4 A5 s0 \<Longrightarrow>
 consecutive s0 s \<Longrightarrow>
-(((((\<not> (w_0 s0)) \<or> ((A5 s) \<or> ((w_0 s) \<and> (A4 s)))) \<and> ((b_1 s0) \<or> ((\<not> (A3 s)) \<or> ((A5 s) \<or> ((w_0 s) \<and> (A4 s)))))) \<and> ((b_1 s) --> (((t > 0) \<or> (\<not> (A1 s))) \<and> ((\<not> (A2 s)) \<or> ((b_0 s0) \<and> ((t1_0 s0) < t)))))) \<and> ((b_0 s) --> ((((t1_0 s) > 0) \<or> (\<not> (A1 s))) \<and> ((\<not> (A2 s)) \<or> ((b_0 s0) \<and> ((t1_0 s0) < (t1_0 s))))))) \<Longrightarrow>
+(((((\<not> (w_0 s0)) \<or> ((A5 s) \<or> ((w_0 s) \<and> (A4 s)))) \<and> ((b_1 s0) \<or> ((\<not> (A3 s)) \<or> ((A5 s) \<or> ((w_0 s) \<and> (A4 s)))))) \<and> ((b_1 s) --> (((t > 0) \<or> (\<not> (A1 s))) \<and> ((\<not> (A2 s)) \<or> ((b_0 s0) \<and> ((((t1_0 s0) = 0) \<and> (\<not> (A1 s))) \<or> ((t1_0 s0) < t))))))) \<and> ((b_0 s) --> ((((t1_0 s) > 0) \<or> (\<not> (A1 s))) \<and> ((\<not> (A2 s)) \<or> ((b_0 s0) \<and> ((((t1_0 s0) = 0) \<and> (\<not> (A1 s))) \<or> ((t1_0 s0) < (t1_0 s)))))))) \<Longrightarrow>
 P6_2_inv_part t b_0 t1_0 b_1 w_0 A1 A2 A3 A4 A5 s"
 
 unfolding P6_2_inv_part_def P6_2_part_def
