examples/Since.thy
@@ -15,7 +15,7 @@ definition dual_since_inv where "dual_since_inv (t::nat) b t1 A1 A2 s \<equiv> b
 
 lemma dual_since_one_point[pastinv]: "dual_since_inv t b t1 A1' A2' s \<Longrightarrow> consecutive s s' \<Longrightarrow>
 b s' \<longrightarrow>(t1 s' > 0 \<or> A2' s' s') \<and> (A1' s' s' \<or> b s \<and> always_imp s (A1' s) (A1' s') \<and>
-always_imp s (A2' s) (A2' s') \<and>  t1 s < t1 s') \<Longrightarrow>
+always_imp s (A2' s) (A2' s') \<and> (t1 s = 0 \<and> A2' s' s' \<or> t1 s < t1 s')) \<Longrightarrow>
 dual_since_inv t b  t1 A1' A2' s' "
   unfolding dual_since_inv_def dual_since_def always_imp_def less_state.simps less_eq_state.simps
   apply(rule impI)
@@ -36,17 +36,25 @@ apply(rule allI)
     apply(rotate_tac -1)
     apply(erule impE)
      apply simp
-    apply(erule allE[of _ r1])
-   apply(subgoal_tac "substate r1 s")
+   apply(erule allE[of _ r1])
+         apply(subgoal_tac "substate r1 s")
     apply(erule impE)
-    apply(simp only: consecutive.simps)
+      apply(erule conjE)
+      apply(rotate_tac -2)
+      apply(erule conjE)
+      apply(rotate_tac -1)
+      apply(erule conjE)
+      apply(rotate_tac -1)
+      apply(erule disjE)
+       apply simp
+      apply(simp only: consecutive.simps)
       apply(rule conjI)
        apply simp
       apply(rule conjI)
        apply simp
       apply(subgoal_tac "t1 s < toEnvNum r1 s'")
     using toEnvNum3[of r1 s s'] apply simp
-    apply simp
+      apply simp
      apply (metis consecutive.simps substate_trans)
     apply (metis consecutive.elims(2) substate_noteq_imp_substate_of_pred)
     done
@@ -55,7 +63,7 @@ apply(rule allI)
 
 lemma dual_since_L7[patternintro]: " dual_since_inv t b t1 A1' A2' s \<Longrightarrow> consecutive s s' \<Longrightarrow>
 (t > 0 \<or> A2' s' s') \<and> (A1' s' s' \<or> b s \<and> always_imp s (A1' s) (A1' s') \<and>
-always_imp s (A2' s) (A2' s') \<and>  t1 s < t) \<Longrightarrow>
+always_imp s (A2' s) (A2' s') \<and>  (t1 s = 0 \<and> A2' s' s' \<or> t1 s < t)) \<Longrightarrow>
 dual_since t A1' A2' s' s' "
   unfolding dual_since_inv_def dual_since_def always_imp_def less_state.simps less_eq_state.simps
   apply(rule allI)
@@ -72,7 +80,15 @@ dual_since t A1' A2' s' s' "
      apply simp
     apply(erule allE[of _ r1])
    apply(subgoal_tac "substate r1 s")
-    apply(erule impE)
+     apply(erule impE)
+      apply(erule conjE)
+      apply(rotate_tac -2)
+      apply(erule conjE)
+      apply(rotate_tac -1)
+      apply(erule conjE)
+      apply(rotate_tac -1)
+      apply(erule disjE)
+       apply simp
     apply(simp only: consecutive.simps)
       apply(rule conjI)
        apply simp
@@ -85,6 +101,8 @@ dual_since t A1' A2' s' s' "
     apply (metis consecutive.elims(2) substate_noteq_imp_substate_of_pred)
     done
   done
+
+
 
 lemma dual_since_L4[invsaving]: "
 consecutive s s' \<Longrightarrow>
