examples/SmartLighting/Requirements.thy
@@ -5,40 +5,89 @@ begin
 definition R1 where "R1 s \<equiv>
 always_part (\<lambda> s1. getVarInt s1 v_timeOfDay' = v_NIGHT' \<longrightarrow> getVarBool s1 v_dayLight' = False \<and> getVarBool s1 v_dimLight' = False) s"
 
+definition Einv1 where "Einv1 s \<equiv> commonExtraInv s \<and>
+always_inv_part (\<lambda> s1. getVarInt s1 v_timeOfDay' = v_NIGHT' \<longrightarrow> getVarBool s1 v_dayLight' = False \<and> getVarBool s1 v_dimLight' = False) s"
+
 definition R2 where "R2 s \<equiv> 
-P4_2_part v_LIGHTING_TIME'TIMEOUT (\<lambda> s1. getVarInt s1 v_timeOfDay' \<noteq> v_NIGHT')
-  (\<lambda> s2. getVarInt s2 v_timeOfDay' \<noteq> v_NIGHT' \<and> getVarBool s2 v_motion' = True \<and> getVarBool s v_light' = v_LOW')
+P4_2_part (v_LIGHTING_TIME'TIMEOUT - 1) (\<lambda> s1. getVarInt s1 v_timeOfDay' \<noteq> v_NIGHT')
+  (\<lambda> s2. getVarInt s2 v_timeOfDay' \<noteq> v_NIGHT' \<and> getVarBool s2 v_motion' = True \<and> getVarBool s2 v_light' = v_LOW')
  (\<lambda> s3. getVarBool s3 v_dayLight' = v_TURNED_ON' \<or> getVarBool s3 v_dimLight' = v_TURNED_ON') (\<lambda> s4. getVarInt s4 v_timeOfDay' = v_NIGHT') s"
 
+definition Einv2 where "Einv2 s \<equiv> commonExtraInv s \<and>
+P4_2_inv_part (v_LIGHTING_TIME'TIMEOUT - 1) 
+  (\<lambda> s. getPstate s p_Lighting' = p_Lighting's_night')
+  (\<lambda> s. if getPstate s p_Lighting' = p_Lighting's_night' \<or> getPstate s p_Motion' \<noteq> p_Motion's_movement' then (v_LIGHTING_TIME'TIMEOUT - 1) 
+    else ltime s p_Motion' - 1)
+  (\<lambda> s1. getVarInt s1 v_timeOfDay' \<noteq> v_NIGHT')
+  (\<lambda> s2. getVarInt s2 v_timeOfDay' \<noteq> v_NIGHT' \<and> getVarBool s2 v_motion' = True \<and> getVarBool s2 v_light' = v_LOW')
+ (\<lambda> s3. getVarBool s3 v_dayLight' = v_TURNED_ON' \<or> getVarBool s3 v_dimLight' = v_TURNED_ON') (\<lambda> s4. getVarInt s4 v_timeOfDay' = v_NIGHT') s"
 
 definition R3 where "R3 s ==
 P2_2_part (v_MORNING_LIGHTING_TIME'TIMEOUT + 1) (\<lambda> s1. getVarInt s1 v_timeOfDay' = v_EARLY_MORNING')
    (\<lambda> s2. getVarInt s2 v_timeOfDay' = v_MORNING_LIGHTING') (\<lambda> s3. getVarBool s3 v_dimLight' = v_TURNED_ON') s"
 
+definition Einv3 where "Einv3 s == commonExtraInv s \<and>
+P2_2_inv_part (v_MORNING_LIGHTING_TIME'TIMEOUT + 1) 
+  (\<lambda> s. getPstate s p_Lighting' \<noteq> p_Lighting's_earlyMorning')
+  (\<lambda> s. if getPstate s p_Lighting' = p_Lighting's_morningLighting' then ltime s p_Lighting' - 1 else v_MORNING_LIGHTING_TIME'TIMEOUT)
+  (\<lambda> s1. getVarInt s1 v_timeOfDay' = v_EARLY_MORNING')
+   (\<lambda> s2. getVarInt s2 v_timeOfDay' = v_MORNING_LIGHTING') (\<lambda> s3. getVarBool s3 v_dimLight' = v_TURNED_ON') s"
+
 definition R4 where "R4 s \<equiv> 
   always2_part (\<lambda> s1. getVarInt s1 v_timeOfDay' = v_DAY') (\<lambda> s2. True) (\<lambda> s2. getVarBool s2 v_dimLight' = False) s"
+
+definition Einv4 where "Einv4 s \<equiv> commonExtraInv s \<and>
+  always2_inv_part (\<lambda> s. getPstate s p_Lighting' \<noteq> p_Lighting's_morningOrDay')
+   (\<lambda> s1. getVarInt s1 v_timeOfDay' = v_DAY') (\<lambda> s2. True) (\<lambda> s2. getVarBool s2 v_dimLight' = False) s"
 
 definition R5 where "R5 s \<equiv> 
 always2_part (\<lambda> s1. getVarInt s1 v_timeOfDay' = v_EVENING') (\<lambda> s2. True) (\<lambda> s2. getVarBool s2 v_dayLight' = False) s"
 
-definition R6 where "R6 s == toEnvP s \<and>
-(\<forall> s1. substate s1 s \<and> toEnvP s1 \<and> getVarBool s1 dayLight' = TURNED_ON' \<longrightarrow> getVarBool s1 dimLight' = TURNED_OFF')"
+definition Einv5 where "Einv5 s \<equiv> commonExtraInv s \<and>
+always2_inv_part (\<lambda> s. getPstate s p_Lighting' \<noteq> p_Lighting's_evening')
+   (\<lambda> s1. getVarInt s1 v_timeOfDay' = v_EVENING') (\<lambda> s2. True) (\<lambda> s2. getVarBool s2 v_dayLight' = False) s"
 
-definition R7 where "R7  s \<equiv> toEnvP s \<and>
-P1 s (LIGHTING_TIME'TIMEOUT + MORNING_LIGHTING_TIME'TIMEOUT) (\<lambda> s1. getVarBool s1 motion' = False)
- (\<lambda> s3. getVarBool s3 dayLight' = False \<and> getVarBool s3 dimLight'= False \<or> getVarBool s3 motion' = True)
-(\<lambda> s2. (getVarBool s2 dayLight' = True \<or> getVarBool s2 dimLight' = True) \<and> getVarBool s2 motion' = False)"
+definition R6 where "R6 s == 
+always_part (\<lambda> s1. \<not> (getVarBool s1 v_dayLight' = v_TURNED_ON' \<and> getVarBool s1 v_dimLight' = v_TURNED_ON')) s"
 
-definition R7_1 where "R7_1 s \<equiv> toEnvP s \<and>
-always s (\<lambda> s1. getVarBool s1 motion' = False \<longrightarrow> constrained_until s1 s (LIGHTING_TIME'TIMEOUT + MORNING_LIGHTING_TIME'TIMEOUT)
-(\<lambda> s2. (getVarBool s2 dayLight' = True \<or> getVarBool s2 dimLight' = True) \<and> getVarBool s2 motion' = False)
- (\<lambda> s3. getVarBool s3 dayLight' = False \<and> getVarBool s3 dimLight'= False \<or> getVarBool s3 motion' = True))"
+definition Einv6 where "Einv6 s == commonExtraInv s \<and>
+always_inv_part (\<lambda> s1. \<not> (getVarBool s1 v_dayLight' = v_TURNED_ON' \<and> getVarBool s1 v_dimLight' = v_TURNED_ON')) s"
 
-definition R8 where "R8 s \<equiv> toEnvP s \<and>
-P1 s (LIGHTING_TIME'TIMEOUT - 1) (\<lambda> s2. P2ex s2 (\<lambda> s1. getVarBool s1 motion' = True \<and> getVarBool s2 motion' = False))
- (\<lambda> s3. getVarBool s3 dayLight' = False \<and> getVarBool s3 dimLight'= False \<or> getVarBool s3 motion' = True \<or>
- P2ex s3 (\<lambda> s2'.  getVarInt s2' timeOfDay' = MORNING_LIGHTING' \<or> getVarInt s3 timeOfDay' = MORNING_LIGHTING'))
-(\<lambda> s2. (getVarBool s2 dayLight' = True \<or> getVarBool s2 dimLight' = True) \<and> getVarBool s2 motion' = False \<and>
- P2all s2 (\<lambda> s1'. getVarInt s1' timeOfDay' \<noteq> MORNING_LIGHTING' \<and>getVarInt s2 timeOfDay' \<noteq> MORNING_LIGHTING'))"
+definition R7 where "R7  s \<equiv> 
+P1_1_part (v_LIGHTING_TIME'TIMEOUT + v_MORNING_LIGHTING_TIME'TIMEOUT) (\<lambda> s1. getVarBool s1 v_motion' = False)
+(\<lambda> s2. (getVarBool s2 v_dayLight' = True \<or> getVarBool s2 v_dimLight' = True) \<and> getVarBool s2 v_motion' = False)
+ (\<lambda> s3. getVarBool s3 v_dayLight' = False \<and> getVarBool s3 v_dimLight'= False \<or> getVarBool s3 v_motion' = True) s"
+
+definition Einv7 where "Einv7  s \<equiv> commonExtraInv s \<and>
+P1_1_inv_part (v_LIGHTING_TIME'TIMEOUT + v_MORNING_LIGHTING_TIME'TIMEOUT)
+  (\<lambda> s. if getPstate s p_Motion' = p_Motion's_movement' then ltime s p_Motion' - 1 
+    else if getPstate s p_Motion' \<noteq> p_Motion's_movement' \<and> getPstate s p_Lighting' = p_Lighting's_morningLighting' 
+      then v_LIGHTING_TIME'TIMEOUT + ltime s p_Lighting' - 1
+    else if getPstate s p_Motion' \<noteq> p_Motion's_movement' \<and> getPstate s p_Lighting' = p_Lighting's_morningOrDay'
+       then v_LIGHTING_TIME'TIMEOUT + v_MORNING_LIGHTING_TIME'TIMEOUT else 0)
+   (\<lambda> s1. getVarBool s1 v_motion' = False)
+(\<lambda> s2. (getVarBool s2 v_dayLight' = True \<or> getVarBool s2 v_dimLight' = True) \<and> getVarBool s2 v_motion' = False)
+ (\<lambda> s3. getVarBool s3 v_dayLight' = False \<and> getVarBool s3 v_dimLight'= False \<or> getVarBool s3 v_motion' = True) s"
+
+definition R8 where "R8 s \<equiv> 
+P1_2_part (v_LIGHTING_TIME'TIMEOUT - 1) (\<lambda> s1. getVarBool s1 v_motion' = True) (\<lambda> s2. getVarBool s2 v_motion' = False)
+(\<lambda> s2. (getVarBool s2 v_dayLight' = True \<or> getVarBool s2 v_dimLight' = True) \<and> getVarBool s2 v_motion' = False \<and>
+   getVarInt s2 v_timeOfDay' \<noteq> v_MORNING_LIGHTING' \<and>
+ (let s1 = pred s2 in toEnvP s1 \<longrightarrow> getVarInt s1 v_timeOfDay' \<noteq> v_MORNING_LIGHTING'))
+ (\<lambda> s3. getVarBool s3 v_dayLight' = False \<and> getVarBool s3 v_dimLight'= False \<or> getVarBool s3 v_motion' = True \<or>
+   getVarInt s3 v_timeOfDay' = v_MORNING_LIGHTING' \<or>
+  (let s2 = pred s3 in toEnvP s2 \<and> getVarInt s2 v_timeOfDay' = v_MORNING_LIGHTING')) s"
+
+definition Einv8 where "Einv8 s \<equiv> commonExtraInv s \<and>
+P1_2_inv_part (v_LIGHTING_TIME'TIMEOUT - 1)
+  (\<lambda> s. getVarBool s v_motion' = False)
+(\<lambda> s. if getPstate s p_Motion' = p_Motion's_movement' then ltime s p_Motion' - 1 else 0)
+   (\<lambda> s1. getVarBool s1 v_motion' = True) (\<lambda> s2. getVarBool s2 v_motion' = False)
+(\<lambda> s2. (getVarBool s2 v_dayLight' = True \<or> getVarBool s2 v_dimLight' = True) \<and> getVarBool s2 v_motion' = False \<and>
+   getVarInt s2 v_timeOfDay' \<noteq> v_MORNING_LIGHTING' \<and>
+ (let s1 = pred s2 in toEnvP s1 \<longrightarrow> getVarInt s1 v_timeOfDay' \<noteq> v_MORNING_LIGHTING'))
+ (\<lambda> s3. getVarBool s3 v_dayLight' = False \<and> getVarBool s3 v_dimLight'= False \<or> getVarBool s3 v_motion' = True \<or>
+   getVarInt s3 v_timeOfDay' = v_MORNING_LIGHTING' \<or>
+  (let s2 = pred s3 in toEnvP s2 \<and> getVarInt s2 v_timeOfDay' = v_MORNING_LIGHTING')) s"
 
 end
